Pack and Chi Base Tables

Examples/Scroll/Keccak/Constants.lean
@@ -7,6 +7,8 @@ namespace Keccak
   def BIT_SIZE: ℕ := 2^BIT_COUNT
   @[keccak_constants] def BIT_SIZE_val: BIT_SIZE = 8 := rfl
   @[keccak_constants] def CHI_BASE_LOOKUP_RANGE: ℕ := 5
+  @[keccak_constants] def CHI_BASE_LOOKUP_TABLE: (Fin 5) → ℕ
+    | 0 => 0 | 1 => 1 | 2 => 1 | 3 => 0 | 4 => 0
   @[keccak_constants] def DEFAULT_KECCAK_ROWS: ℕ := 12
   @[keccak_constants] def KECCAK_DEGREE: ℕ := 10 -- environment variable during run
   @[keccak_constants] def MAX_DEGREE: ℕ := 9
