Examples/Scroll/Keccak/Lookups/All.lean
@@ -1,4 +1,6 @@
 import Examples.Scroll.Keccak.Lookups.Columns
+import Examples.Scroll.Keccak.Lookups.ChiBase.All
 import Examples.Scroll.Keccak.Lookups.Normalize_3.All
 import Examples.Scroll.Keccak.Lookups.Normalize_4.All
 import Examples.Scroll.Keccak.Lookups.Normalize_6.All
+import Examples.Scroll.Keccak.Lookups.PackTable.All
