Examples/Scroll/Keccak/Lookups/ChiBase/Input.lean
@@ -1,0 +1,244 @@
+import Examples.Scroll.Keccak.Constants
+import Examples.Scroll.Keccak.Spec.KeccakConstants
+
+namespace Keccak.Lookups.ChiBase
+  -- columns 14 and 15
+  -- def part_size := get_num_bits_per_base_chi_lookup
+
+  -- the number of args to input and output
+  -- lemma part_size_val: part_size = 4 := by simp [part_size, keccak_constants]
+
+  def input (P: ℕ) (x0 x1 x2 x3: ℕ): ZMod P :=
+    ↑(([x0, x1, x2, x3].foldl (
+      λ (⟨input, factor⟩: ℕ × ℕ) (input_part: ℕ) =>
+        (input + input_part*factor, factor * BIT_SIZE)
+    ) (0, 1): ℕ × ℕ).1)
+
+  def input_by_row (P: ℕ) (row: ℕ) : ZMod P :=
+    input P ((row / 125) % 5) ((row / 25) % 5) ((row / 5) % 5) (row % 5)
+
+  lemma input_eval: input P x0 x1 x2 x3 =
+    x0 +
+    x1*BIT_SIZE +
+    x2*BIT_SIZE^2 +
+    x3*BIT_SIZE^3
+    := by
+      simp [input, ←pow_two, ←Nat.pow_add_one, keccak_constants]
+      norm_num
+
+  lemma fixed_func_col_14_0_to_9_input (c: ValidCircuit P P_Prime) (n: Finset.Ico 0 10): fixed_func_col_14 c n = input_by_row P n := by
+    fin_cases n <;> simp [fixed_func_col_14, fixed_func_col_14_0_to_621, fixed_func_col_14_0_to_99, fixed_func_col_14_0_to_9, input_by_row, input, keccak_constants]
+  lemma fixed_func_col_14_10_to_19_input (c: ValidCircuit P P_Prime) (n: Finset.Ico 10 20): fixed_func_col_14 c n = input_by_row P n := by
+    fin_cases n <;> simp [fixed_func_col_14, fixed_func_col_14_0_to_621, fixed_func_col_14_0_to_99, fixed_func_col_14_10_to_19, input_by_row, input, keccak_constants]
+  lemma fixed_func_col_14_20_to_29_input (c: ValidCircuit P P_Prime) (n: Finset.Ico 20 30): fixed_func_col_14 c n = input_by_row P n := by
+    fin_cases n <;> simp [fixed_func_col_14, fixed_func_col_14_0_to_621, fixed_func_col_14_0_to_99, fixed_func_col_14_20_to_29, input_by_row, input, keccak_constants]
+  lemma fixed_func_col_14_30_to_39_input (c: ValidCircuit P P_Prime) (n: Finset.Ico 30 40): fixed_func_col_14 c n = input_by_row P n := by
+    fin_cases n <;> simp [fixed_func_col_14, fixed_func_col_14_0_to_621, fixed_func_col_14_0_to_99, fixed_func_col_14_30_to_39, input_by_row, input, keccak_constants]
+  lemma fixed_func_col_14_40_to_49_input (c: ValidCircuit P P_Prime) (n: Finset.Ico 40 50): fixed_func_col_14 c n = input_by_row P n := by
+    fin_cases n <;> simp [fixed_func_col_14, fixed_func_col_14_0_to_621, fixed_func_col_14_0_to_99, fixed_func_col_14_40_to_49, input_by_row, input, keccak_constants]
+  lemma fixed_func_col_14_50_to_59_input (c: ValidCircuit P P_Prime) (n: Finset.Ico 50 60): fixed_func_col_14 c n = input_by_row P n := by
+    fin_cases n <;> simp [fixed_func_col_14, fixed_func_col_14_0_to_621, fixed_func_col_14_0_to_99, fixed_func_col_14_50_to_59, input_by_row, input, keccak_constants]
+  lemma fixed_func_col_14_60_to_69_input (c: ValidCircuit P P_Prime) (n: Finset.Ico 60 70): fixed_func_col_14 c n = input_by_row P n := by
+    fin_cases n <;> simp [fixed_func_col_14, fixed_func_col_14_0_to_621, fixed_func_col_14_0_to_99, fixed_func_col_14_60_to_69, input_by_row, input, keccak_constants]
+  lemma fixed_func_col_14_70_to_79_input (c: ValidCircuit P P_Prime) (n: Finset.Ico 70 80): fixed_func_col_14 c n = input_by_row P n := by
+    fin_cases n <;> simp [fixed_func_col_14, fixed_func_col_14_0_to_621, fixed_func_col_14_0_to_99, fixed_func_col_14_70_to_79, input_by_row, input, keccak_constants]
+  lemma fixed_func_col_14_80_to_89_input (c: ValidCircuit P P_Prime) (n: Finset.Ico 80 90): fixed_func_col_14 c n = input_by_row P n := by
+    fin_cases n <;> simp [fixed_func_col_14, fixed_func_col_14_0_to_621, fixed_func_col_14_0_to_99, fixed_func_col_14_80_to_89, input_by_row, input, keccak_constants]
+  lemma fixed_func_col_14_90_to_99_input (c: ValidCircuit P P_Prime) (n: Finset.Ico 90 100): fixed_func_col_14 c n = input_by_row P n := by
+    fin_cases n <;> simp [fixed_func_col_14, fixed_func_col_14_0_to_621, fixed_func_col_14_0_to_99, fixed_func_col_14_90_to_99, input_by_row, input, keccak_constants]
+  lemma fixed_func_col_14_100_to_109_input (c: ValidCircuit P P_Prime) (n: Finset.Ico 100 110): fixed_func_col_14 c n = input_by_row P n := by
+    fin_cases n <;> simp [fixed_func_col_14, fixed_func_col_14_0_to_621, fixed_func_col_14_100_to_199, fixed_func_col_14_100_to_109, input_by_row, input, keccak_constants]
+  lemma fixed_func_col_14_110_to_119_input (c: ValidCircuit P P_Prime) (n: Finset.Ico 110 120): fixed_func_col_14 c n = input_by_row P n := by
+    fin_cases n <;> simp [fixed_func_col_14, fixed_func_col_14_0_to_621, fixed_func_col_14_100_to_199, fixed_func_col_14_110_to_119, input_by_row, input, keccak_constants]
+  lemma fixed_func_col_14_120_to_129_input (c: ValidCircuit P P_Prime) (n: Finset.Ico 120 130): fixed_func_col_14 c n = input_by_row P n := by
+    fin_cases n <;> simp [fixed_func_col_14, fixed_func_col_14_0_to_621, fixed_func_col_14_100_to_199, fixed_func_col_14_120_to_129, input_by_row, input, keccak_constants]
+  lemma fixed_func_col_14_130_to_139_input (c: ValidCircuit P P_Prime) (n: Finset.Ico 130 140): fixed_func_col_14 c n = input_by_row P n := by
+    fin_cases n <;> simp [fixed_func_col_14, fixed_func_col_14_0_to_621, fixed_func_col_14_100_to_199, fixed_func_col_14_130_to_139, input_by_row, input, keccak_constants]
+  lemma fixed_func_col_14_140_to_149_input (c: ValidCircuit P P_Prime) (n: Finset.Ico 140 150): fixed_func_col_14 c n = input_by_row P n := by
+    fin_cases n <;> simp [fixed_func_col_14, fixed_func_col_14_0_to_621, fixed_func_col_14_100_to_199, fixed_func_col_14_140_to_149, input_by_row, input, keccak_constants]
+  lemma fixed_func_col_14_150_to_159_input (c: ValidCircuit P P_Prime) (n: Finset.Ico 150 160): fixed_func_col_14 c n = input_by_row P n := by
+    fin_cases n <;> simp [fixed_func_col_14, fixed_func_col_14_0_to_621, fixed_func_col_14_100_to_199, fixed_func_col_14_150_to_159, input_by_row, input, keccak_constants]
+  lemma fixed_func_col_14_160_to_169_input (c: ValidCircuit P P_Prime) (n: Finset.Ico 160 170): fixed_func_col_14 c n = input_by_row P n := by
+    fin_cases n <;> simp [fixed_func_col_14, fixed_func_col_14_0_to_621, fixed_func_col_14_100_to_199, fixed_func_col_14_160_to_169, input_by_row, input, keccak_constants]
+  lemma fixed_func_col_14_170_to_179_input (c: ValidCircuit P P_Prime) (n: Finset.Ico 170 180): fixed_func_col_14 c n = input_by_row P n := by
+    fin_cases n <;> simp [fixed_func_col_14, fixed_func_col_14_0_to_621, fixed_func_col_14_100_to_199, fixed_func_col_14_170_to_179, input_by_row, input, keccak_constants]
+  lemma fixed_func_col_14_180_to_189_input (c: ValidCircuit P P_Prime) (n: Finset.Ico 180 190): fixed_func_col_14 c n = input_by_row P n := by
+    fin_cases n <;> simp [fixed_func_col_14, fixed_func_col_14_0_to_621, fixed_func_col_14_100_to_199, fixed_func_col_14_180_to_189, input_by_row, input, keccak_constants]
+  lemma fixed_func_col_14_190_to_199_input (c: ValidCircuit P P_Prime) (n: Finset.Ico 190 200): fixed_func_col_14 c n = input_by_row P n := by
+    fin_cases n <;> simp [fixed_func_col_14, fixed_func_col_14_0_to_621, fixed_func_col_14_100_to_199, fixed_func_col_14_190_to_199, input_by_row, input, keccak_constants]
+  lemma fixed_func_col_14_200_to_209_input (c: ValidCircuit P P_Prime) (n: Finset.Ico 200 210): fixed_func_col_14 c n = input_by_row P n := by
+    fin_cases n <;> simp [fixed_func_col_14, fixed_func_col_14_0_to_621, fixed_func_col_14_200_to_299, fixed_func_col_14_200_to_209, input_by_row, input, keccak_constants]
+  lemma fixed_func_col_14_210_to_219_input (c: ValidCircuit P P_Prime) (n: Finset.Ico 210 220): fixed_func_col_14 c n = input_by_row P n := by
+    fin_cases n <;> simp [fixed_func_col_14, fixed_func_col_14_0_to_621, fixed_func_col_14_200_to_299, fixed_func_col_14_210_to_219, input_by_row, input, keccak_constants]
+  lemma fixed_func_col_14_220_to_229_input (c: ValidCircuit P P_Prime) (n: Finset.Ico 220 230): fixed_func_col_14 c n = input_by_row P n := by
+    fin_cases n <;> simp [fixed_func_col_14, fixed_func_col_14_0_to_621, fixed_func_col_14_200_to_299, fixed_func_col_14_220_to_229, input_by_row, input, keccak_constants]
+  lemma fixed_func_col_14_230_to_239_input (c: ValidCircuit P P_Prime) (n: Finset.Ico 230 240): fixed_func_col_14 c n = input_by_row P n := by
+    fin_cases n <;> simp [fixed_func_col_14, fixed_func_col_14_0_to_621, fixed_func_col_14_200_to_299, fixed_func_col_14_230_to_239, input_by_row, input, keccak_constants]
+  lemma fixed_func_col_14_240_to_249_input (c: ValidCircuit P P_Prime) (n: Finset.Ico 240 250): fixed_func_col_14 c n = input_by_row P n := by
+    fin_cases n <;> simp [fixed_func_col_14, fixed_func_col_14_0_to_621, fixed_func_col_14_200_to_299, fixed_func_col_14_240_to_249, input_by_row, input, keccak_constants]
+  lemma fixed_func_col_14_250_to_259_input (c: ValidCircuit P P_Prime) (n: Finset.Ico 250 260): fixed_func_col_14 c n = input_by_row P n := by
+    fin_cases n <;> simp [fixed_func_col_14, fixed_func_col_14_0_to_621, fixed_func_col_14_200_to_299, fixed_func_col_14_250_to_259, input_by_row, input, keccak_constants]
+  lemma fixed_func_col_14_260_to_269_input (c: ValidCircuit P P_Prime) (n: Finset.Ico 260 270): fixed_func_col_14 c n = input_by_row P n := by
+    fin_cases n <;> simp [fixed_func_col_14, fixed_func_col_14_0_to_621, fixed_func_col_14_200_to_299, fixed_func_col_14_260_to_269, input_by_row, input, keccak_constants]
+  lemma fixed_func_col_14_270_to_279_input (c: ValidCircuit P P_Prime) (n: Finset.Ico 270 280): fixed_func_col_14 c n = input_by_row P n := by
+    fin_cases n <;> simp [fixed_func_col_14, fixed_func_col_14_0_to_621, fixed_func_col_14_200_to_299, fixed_func_col_14_270_to_279, input_by_row, input, keccak_constants]
+  lemma fixed_func_col_14_280_to_289_input (c: ValidCircuit P P_Prime) (n: Finset.Ico 280 290): fixed_func_col_14 c n = input_by_row P n := by
+    fin_cases n <;> simp [fixed_func_col_14, fixed_func_col_14_0_to_621, fixed_func_col_14_200_to_299, fixed_func_col_14_280_to_289, input_by_row, input, keccak_constants]
+  lemma fixed_func_col_14_290_to_299_input (c: ValidCircuit P P_Prime) (n: Finset.Ico 290 300): fixed_func_col_14 c n = input_by_row P n := by
+    fin_cases n <;> simp [fixed_func_col_14, fixed_func_col_14_0_to_621, fixed_func_col_14_200_to_299, fixed_func_col_14_290_to_299, input_by_row, input, keccak_constants]
+  lemma fixed_func_col_14_300_to_309_input (c: ValidCircuit P P_Prime) (n: Finset.Ico 300 310): fixed_func_col_14 c n = input_by_row P n := by
+    fin_cases n <;> simp [fixed_func_col_14, fixed_func_col_14_0_to_621, fixed_func_col_14_300_to_399, fixed_func_col_14_300_to_309, input_by_row, input, keccak_constants]
+  lemma fixed_func_col_14_310_to_319_input (c: ValidCircuit P P_Prime) (n: Finset.Ico 310 320): fixed_func_col_14 c n = input_by_row P n := by
+    fin_cases n <;> simp [fixed_func_col_14, fixed_func_col_14_0_to_621, fixed_func_col_14_300_to_399, fixed_func_col_14_310_to_319, input_by_row, input, keccak_constants]
+  lemma fixed_func_col_14_320_to_329_input (c: ValidCircuit P P_Prime) (n: Finset.Ico 320 330): fixed_func_col_14 c n = input_by_row P n := by
+    fin_cases n <;> simp [fixed_func_col_14, fixed_func_col_14_0_to_621, fixed_func_col_14_300_to_399, fixed_func_col_14_320_to_329, input_by_row, input, keccak_constants]
+  lemma fixed_func_col_14_330_to_339_input (c: ValidCircuit P P_Prime) (n: Finset.Ico 330 340): fixed_func_col_14 c n = input_by_row P n := by
+    fin_cases n <;> simp [fixed_func_col_14, fixed_func_col_14_0_to_621, fixed_func_col_14_300_to_399, fixed_func_col_14_330_to_339, input_by_row, input, keccak_constants]
+  lemma fixed_func_col_14_340_to_349_input (c: ValidCircuit P P_Prime) (n: Finset.Ico 340 350): fixed_func_col_14 c n = input_by_row P n := by
+    fin_cases n <;> simp [fixed_func_col_14, fixed_func_col_14_0_to_621, fixed_func_col_14_300_to_399, fixed_func_col_14_340_to_349, input_by_row, input, keccak_constants]
+  lemma fixed_func_col_14_350_to_359_input (c: ValidCircuit P P_Prime) (n: Finset.Ico 350 360): fixed_func_col_14 c n = input_by_row P n := by
+    fin_cases n <;> simp [fixed_func_col_14, fixed_func_col_14_0_to_621, fixed_func_col_14_300_to_399, fixed_func_col_14_350_to_359, input_by_row, input, keccak_constants]
+  lemma fixed_func_col_14_360_to_369_input (c: ValidCircuit P P_Prime) (n: Finset.Ico 360 370): fixed_func_col_14 c n = input_by_row P n := by
+    fin_cases n <;> simp [fixed_func_col_14, fixed_func_col_14_0_to_621, fixed_func_col_14_300_to_399, fixed_func_col_14_360_to_369, input_by_row, input, keccak_constants]
+  lemma fixed_func_col_14_370_to_379_input (c: ValidCircuit P P_Prime) (n: Finset.Ico 370 380): fixed_func_col_14 c n = input_by_row P n := by
+    fin_cases n <;> simp [fixed_func_col_14, fixed_func_col_14_0_to_621, fixed_func_col_14_300_to_399, fixed_func_col_14_370_to_379, input_by_row, input, keccak_constants]
+  lemma fixed_func_col_14_380_to_389_input (c: ValidCircuit P P_Prime) (n: Finset.Ico 380 390): fixed_func_col_14 c n = input_by_row P n := by
+    fin_cases n <;> simp [fixed_func_col_14, fixed_func_col_14_0_to_621, fixed_func_col_14_300_to_399, fixed_func_col_14_380_to_389, input_by_row, input, keccak_constants]
+  lemma fixed_func_col_14_390_to_399_input (c: ValidCircuit P P_Prime) (n: Finset.Ico 390 400): fixed_func_col_14 c n = input_by_row P n := by
+    fin_cases n <;> simp [fixed_func_col_14, fixed_func_col_14_0_to_621, fixed_func_col_14_300_to_399, fixed_func_col_14_390_to_399, input_by_row, input, keccak_constants]
+  lemma fixed_func_col_14_400_to_409_input (c: ValidCircuit P P_Prime) (n: Finset.Ico 400 410): fixed_func_col_14 c n = input_by_row P n := by
+    fin_cases n <;> simp [fixed_func_col_14, fixed_func_col_14_0_to_621, fixed_func_col_14_400_to_499, fixed_func_col_14_400_to_409, input_by_row, input, keccak_constants]
+  lemma fixed_func_col_14_410_to_419_input (c: ValidCircuit P P_Prime) (n: Finset.Ico 410 420): fixed_func_col_14 c n = input_by_row P n := by
+    fin_cases n <;> simp [fixed_func_col_14, fixed_func_col_14_0_to_621, fixed_func_col_14_400_to_499, fixed_func_col_14_410_to_419, input_by_row, input, keccak_constants]
+  lemma fixed_func_col_14_420_to_429_input (c: ValidCircuit P P_Prime) (n: Finset.Ico 420 430): fixed_func_col_14 c n = input_by_row P n := by
+    fin_cases n <;> simp [fixed_func_col_14, fixed_func_col_14_0_to_621, fixed_func_col_14_400_to_499, fixed_func_col_14_420_to_429, input_by_row, input, keccak_constants]
+  lemma fixed_func_col_14_430_to_439_input (c: ValidCircuit P P_Prime) (n: Finset.Ico 430 440): fixed_func_col_14 c n = input_by_row P n := by
+    fin_cases n <;> simp [fixed_func_col_14, fixed_func_col_14_0_to_621, fixed_func_col_14_400_to_499, fixed_func_col_14_430_to_439, input_by_row, input, keccak_constants]
+  lemma fixed_func_col_14_440_to_449_input (c: ValidCircuit P P_Prime) (n: Finset.Ico 440 450): fixed_func_col_14 c n = input_by_row P n := by
+    fin_cases n <;> simp [fixed_func_col_14, fixed_func_col_14_0_to_621, fixed_func_col_14_400_to_499, fixed_func_col_14_440_to_449, input_by_row, input, keccak_constants]
+  lemma fixed_func_col_14_450_to_459_input (c: ValidCircuit P P_Prime) (n: Finset.Ico 450 460): fixed_func_col_14 c n = input_by_row P n := by
+    fin_cases n <;> simp [fixed_func_col_14, fixed_func_col_14_0_to_621, fixed_func_col_14_400_to_499, fixed_func_col_14_450_to_459, input_by_row, input, keccak_constants]
+  lemma fixed_func_col_14_460_to_469_input (c: ValidCircuit P P_Prime) (n: Finset.Ico 460 470): fixed_func_col_14 c n = input_by_row P n := by
+    fin_cases n <;> simp [fixed_func_col_14, fixed_func_col_14_0_to_621, fixed_func_col_14_400_to_499, fixed_func_col_14_460_to_469, input_by_row, input, keccak_constants]
+  lemma fixed_func_col_14_470_to_479_input (c: ValidCircuit P P_Prime) (n: Finset.Ico 470 480): fixed_func_col_14 c n = input_by_row P n := by
+    fin_cases n <;> simp [fixed_func_col_14, fixed_func_col_14_0_to_621, fixed_func_col_14_400_to_499, fixed_func_col_14_470_to_479, input_by_row, input, keccak_constants]
+  lemma fixed_func_col_14_480_to_489_input (c: ValidCircuit P P_Prime) (n: Finset.Ico 480 490): fixed_func_col_14 c n = input_by_row P n := by
+    fin_cases n <;> simp [fixed_func_col_14, fixed_func_col_14_0_to_621, fixed_func_col_14_400_to_499, fixed_func_col_14_480_to_489, input_by_row, input, keccak_constants]
+  lemma fixed_func_col_14_490_to_499_input (c: ValidCircuit P P_Prime) (n: Finset.Ico 490 500): fixed_func_col_14 c n = input_by_row P n := by
+    fin_cases n <;> simp [fixed_func_col_14, fixed_func_col_14_0_to_621, fixed_func_col_14_400_to_499, fixed_func_col_14_490_to_499, input_by_row, input, keccak_constants]
+  lemma fixed_func_col_14_500_to_509_input (c: ValidCircuit P P_Prime) (n: Finset.Ico 500 510): fixed_func_col_14 c n = input_by_row P n := by
+    fin_cases n <;> simp [fixed_func_col_14, fixed_func_col_14_0_to_621, fixed_func_col_14_500_to_599, fixed_func_col_14_500_to_509, input_by_row, input, keccak_constants]
+  lemma fixed_func_col_14_510_to_519_input (c: ValidCircuit P P_Prime) (n: Finset.Ico 510 520): fixed_func_col_14 c n = input_by_row P n := by
+    fin_cases n <;> simp [fixed_func_col_14, fixed_func_col_14_0_to_621, fixed_func_col_14_500_to_599, fixed_func_col_14_510_to_519, input_by_row, input, keccak_constants]
+  lemma fixed_func_col_14_520_to_529_input (c: ValidCircuit P P_Prime) (n: Finset.Ico 520 530): fixed_func_col_14 c n = input_by_row P n := by
+    fin_cases n <;> simp [fixed_func_col_14, fixed_func_col_14_0_to_621, fixed_func_col_14_500_to_599, fixed_func_col_14_520_to_529, input_by_row, input, keccak_constants]
+  lemma fixed_func_col_14_530_to_539_input (c: ValidCircuit P P_Prime) (n: Finset.Ico 530 540): fixed_func_col_14 c n = input_by_row P n := by
+    fin_cases n <;> simp [fixed_func_col_14, fixed_func_col_14_0_to_621, fixed_func_col_14_500_to_599, fixed_func_col_14_530_to_539, input_by_row, input, keccak_constants]
+  lemma fixed_func_col_14_540_to_549_input (c: ValidCircuit P P_Prime) (n: Finset.Ico 540 550): fixed_func_col_14 c n = input_by_row P n := by
+    fin_cases n <;> simp [fixed_func_col_14, fixed_func_col_14_0_to_621, fixed_func_col_14_500_to_599, fixed_func_col_14_540_to_549, input_by_row, input, keccak_constants]
+  lemma fixed_func_col_14_550_to_559_input (c: ValidCircuit P P_Prime) (n: Finset.Ico 550 560): fixed_func_col_14 c n = input_by_row P n := by
+    fin_cases n <;> simp [fixed_func_col_14, fixed_func_col_14_0_to_621, fixed_func_col_14_500_to_599, fixed_func_col_14_550_to_559, input_by_row, input, keccak_constants]
+  lemma fixed_func_col_14_560_to_569_input (c: ValidCircuit P P_Prime) (n: Finset.Ico 560 570): fixed_func_col_14 c n = input_by_row P n := by
+    fin_cases n <;> simp [fixed_func_col_14, fixed_func_col_14_0_to_621, fixed_func_col_14_500_to_599, fixed_func_col_14_560_to_569, input_by_row, input, keccak_constants]
+  lemma fixed_func_col_14_570_to_579_input (c: ValidCircuit P P_Prime) (n: Finset.Ico 570 580): fixed_func_col_14 c n = input_by_row P n := by
+    fin_cases n <;> simp [fixed_func_col_14, fixed_func_col_14_0_to_621, fixed_func_col_14_500_to_599, fixed_func_col_14_570_to_579, input_by_row, input, keccak_constants]
+  lemma fixed_func_col_14_580_to_589_input (c: ValidCircuit P P_Prime) (n: Finset.Ico 580 590): fixed_func_col_14 c n = input_by_row P n := by
+    fin_cases n <;> simp [fixed_func_col_14, fixed_func_col_14_0_to_621, fixed_func_col_14_500_to_599, fixed_func_col_14_580_to_589, input_by_row, input, keccak_constants]
+  lemma fixed_func_col_14_590_to_599_input (c: ValidCircuit P P_Prime) (n: Finset.Ico 590 600): fixed_func_col_14 c n = input_by_row P n := by
+    fin_cases n <;> simp [fixed_func_col_14, fixed_func_col_14_0_to_621, fixed_func_col_14_500_to_599, fixed_func_col_14_590_to_599, input_by_row, input, keccak_constants]
+  lemma fixed_func_col_14_600_to_609_input (c: ValidCircuit P P_Prime) (n: Finset.Ico 600 610): fixed_func_col_14 c n = input_by_row P n := by
+    fin_cases n <;> simp [fixed_func_col_14, fixed_func_col_14_0_to_621, fixed_func_col_14_600_to_609, input_by_row, input, keccak_constants]
+  lemma fixed_func_col_14_610_to_619_input (c: ValidCircuit P P_Prime) (n: Finset.Ico 610 620): fixed_func_col_14 c n = input_by_row P n := by
+    fin_cases n <;> simp [fixed_func_col_14, fixed_func_col_14_0_to_621, fixed_func_col_14_610_to_619, input_by_row, input, keccak_constants]
+  lemma fixed_func_col_14_620_to_624_input (c: ValidCircuit P P_Prime) (n: Finset.Ico 620 625): fixed_func_col_14 c n = input_by_row P n := by
+    fin_cases n <;> simp [fixed_func_col_14, fixed_func_col_14_0_to_621, input_by_row, input, keccak_constants]
+
+  lemma fixed_func_col_14_0_to_624_input (c : ValidCircuit P P_Prime) (n : Fin 625) :
+    fixed_func_col_14 c n = input_by_row P n := by
+      rcases n with ⟨n, hn⟩
+      by_cases h100: n < 100
+      . by_cases h10: n < 10; exact fixed_func_col_14_0_to_9_input c ⟨n, Finset.mem_Ico.mpr ⟨(Nat.zero_le n), h10⟩⟩
+        by_cases h20: n < 20; exact fixed_func_col_14_10_to_19_input c ⟨n, Finset.mem_Ico.mpr ⟨Nat.le_of_not_lt h10, h20⟩⟩
+        by_cases h30: n < 30; exact fixed_func_col_14_20_to_29_input c ⟨n, Finset.mem_Ico.mpr ⟨Nat.le_of_not_lt h20, h30⟩⟩
+        by_cases h40: n < 40; exact fixed_func_col_14_30_to_39_input c ⟨n, Finset.mem_Ico.mpr ⟨Nat.le_of_not_lt h30, h40⟩⟩
+        by_cases h50: n < 50; exact fixed_func_col_14_40_to_49_input c ⟨n, Finset.mem_Ico.mpr ⟨Nat.le_of_not_lt h40, h50⟩⟩
+        by_cases h60: n < 60; exact fixed_func_col_14_50_to_59_input c ⟨n, Finset.mem_Ico.mpr ⟨Nat.le_of_not_lt h50, h60⟩⟩
+        by_cases h70: n < 70; exact fixed_func_col_14_60_to_69_input c ⟨n, Finset.mem_Ico.mpr ⟨Nat.le_of_not_lt h60, h70⟩⟩
+        by_cases h80: n < 80; exact fixed_func_col_14_70_to_79_input c ⟨n, Finset.mem_Ico.mpr ⟨Nat.le_of_not_lt h70, h80⟩⟩
+        by_cases h90: n < 90; exact fixed_func_col_14_80_to_89_input c ⟨n, Finset.mem_Ico.mpr ⟨Nat.le_of_not_lt h80, h90⟩⟩
+        exact fixed_func_col_14_90_to_99_input c ⟨n, Finset.mem_Ico.mpr ⟨Nat.le_of_not_lt h90, h100⟩⟩
+      by_cases h200: n < 200
+      . by_cases h110: n < 110; exact fixed_func_col_14_100_to_109_input c ⟨n, Finset.mem_Ico.mpr ⟨Nat.le_of_not_lt h100, h110⟩⟩
+        by_cases h120: n < 120; exact fixed_func_col_14_110_to_119_input c ⟨n, Finset.mem_Ico.mpr ⟨Nat.le_of_not_lt h110, h120⟩⟩
+        by_cases h130: n < 130; exact fixed_func_col_14_120_to_129_input c ⟨n, Finset.mem_Ico.mpr ⟨Nat.le_of_not_lt h120, h130⟩⟩
+        by_cases h140: n < 140; exact fixed_func_col_14_130_to_139_input c ⟨n, Finset.mem_Ico.mpr ⟨Nat.le_of_not_lt h130, h140⟩⟩
+        by_cases h150: n < 150; exact fixed_func_col_14_140_to_149_input c ⟨n, Finset.mem_Ico.mpr ⟨Nat.le_of_not_lt h140, h150⟩⟩
+        by_cases h160: n < 160; exact fixed_func_col_14_150_to_159_input c ⟨n, Finset.mem_Ico.mpr ⟨Nat.le_of_not_lt h150, h160⟩⟩
+        by_cases h170: n < 170; exact fixed_func_col_14_160_to_169_input c ⟨n, Finset.mem_Ico.mpr ⟨Nat.le_of_not_lt h160, h170⟩⟩
+        by_cases h180: n < 180; exact fixed_func_col_14_170_to_179_input c ⟨n, Finset.mem_Ico.mpr ⟨Nat.le_of_not_lt h170, h180⟩⟩
+        by_cases h190: n < 190; exact fixed_func_col_14_180_to_189_input c ⟨n, Finset.mem_Ico.mpr ⟨Nat.le_of_not_lt h180, h190⟩⟩
+        exact fixed_func_col_14_190_to_199_input c ⟨n, Finset.mem_Ico.mpr ⟨Nat.le_of_not_lt h190, h200⟩⟩
+      by_cases h300: n < 300
+      . by_cases h210: n < 210; exact fixed_func_col_14_200_to_209_input c ⟨n, Finset.mem_Ico.mpr ⟨Nat.le_of_not_lt h200, h210⟩⟩
+        by_cases h220: n < 220; exact fixed_func_col_14_210_to_219_input c ⟨n, Finset.mem_Ico.mpr ⟨Nat.le_of_not_lt h210, h220⟩⟩
+        by_cases h230: n < 230; exact fixed_func_col_14_220_to_229_input c ⟨n, Finset.mem_Ico.mpr ⟨Nat.le_of_not_lt h220, h230⟩⟩
+        by_cases h240: n < 240; exact fixed_func_col_14_230_to_239_input c ⟨n, Finset.mem_Ico.mpr ⟨Nat.le_of_not_lt h230, h240⟩⟩
+        by_cases h250: n < 250; exact fixed_func_col_14_240_to_249_input c ⟨n, Finset.mem_Ico.mpr ⟨Nat.le_of_not_lt h240, h250⟩⟩
+        by_cases h260: n < 260; exact fixed_func_col_14_250_to_259_input c ⟨n, Finset.mem_Ico.mpr ⟨Nat.le_of_not_lt h250, h260⟩⟩
+        by_cases h270: n < 270; exact fixed_func_col_14_260_to_269_input c ⟨n, Finset.mem_Ico.mpr ⟨Nat.le_of_not_lt h260, h270⟩⟩
+        by_cases h280: n < 280; exact fixed_func_col_14_270_to_279_input c ⟨n, Finset.mem_Ico.mpr ⟨Nat.le_of_not_lt h270, h280⟩⟩
+        by_cases h290: n < 290; exact fixed_func_col_14_280_to_289_input c ⟨n, Finset.mem_Ico.mpr ⟨Nat.le_of_not_lt h280, h290⟩⟩
+        exact fixed_func_col_14_290_to_299_input c ⟨n, Finset.mem_Ico.mpr ⟨Nat.le_of_not_lt h290, h300⟩⟩
+      by_cases h400: n < 400
+      . by_cases h310: n < 310; exact fixed_func_col_14_300_to_309_input c ⟨n, Finset.mem_Ico.mpr ⟨Nat.le_of_not_lt h300, h310⟩⟩
+        by_cases h320: n < 320; exact fixed_func_col_14_310_to_319_input c ⟨n, Finset.mem_Ico.mpr ⟨Nat.le_of_not_lt h310, h320⟩⟩
+        by_cases h330: n < 330; exact fixed_func_col_14_320_to_329_input c ⟨n, Finset.mem_Ico.mpr ⟨Nat.le_of_not_lt h320, h330⟩⟩
+        by_cases h340: n < 340; exact fixed_func_col_14_330_to_339_input c ⟨n, Finset.mem_Ico.mpr ⟨Nat.le_of_not_lt h330, h340⟩⟩
+        by_cases h350: n < 350; exact fixed_func_col_14_340_to_349_input c ⟨n, Finset.mem_Ico.mpr ⟨Nat.le_of_not_lt h340, h350⟩⟩
+        by_cases h360: n < 360; exact fixed_func_col_14_350_to_359_input c ⟨n, Finset.mem_Ico.mpr ⟨Nat.le_of_not_lt h350, h360⟩⟩
+        by_cases h370: n < 370; exact fixed_func_col_14_360_to_369_input c ⟨n, Finset.mem_Ico.mpr ⟨Nat.le_of_not_lt h360, h370⟩⟩
+        by_cases h380: n < 380; exact fixed_func_col_14_370_to_379_input c ⟨n, Finset.mem_Ico.mpr ⟨Nat.le_of_not_lt h370, h380⟩⟩
+        by_cases h390: n < 390; exact fixed_func_col_14_380_to_389_input c ⟨n, Finset.mem_Ico.mpr ⟨Nat.le_of_not_lt h380, h390⟩⟩
+        exact fixed_func_col_14_390_to_399_input c ⟨n, Finset.mem_Ico.mpr ⟨Nat.le_of_not_lt h390, h400⟩⟩
+      by_cases h500: n < 500
+      . by_cases h410: n < 410; exact fixed_func_col_14_400_to_409_input c ⟨n, Finset.mem_Ico.mpr ⟨Nat.le_of_not_lt h400, h410⟩⟩
+        by_cases h420: n < 420; exact fixed_func_col_14_410_to_419_input c ⟨n, Finset.mem_Ico.mpr ⟨Nat.le_of_not_lt h410, h420⟩⟩
+        by_cases h430: n < 430; exact fixed_func_col_14_420_to_429_input c ⟨n, Finset.mem_Ico.mpr ⟨Nat.le_of_not_lt h420, h430⟩⟩
+        by_cases h440: n < 440; exact fixed_func_col_14_430_to_439_input c ⟨n, Finset.mem_Ico.mpr ⟨Nat.le_of_not_lt h430, h440⟩⟩
+        by_cases h450: n < 450; exact fixed_func_col_14_440_to_449_input c ⟨n, Finset.mem_Ico.mpr ⟨Nat.le_of_not_lt h440, h450⟩⟩
+        by_cases h460: n < 460; exact fixed_func_col_14_450_to_459_input c ⟨n, Finset.mem_Ico.mpr ⟨Nat.le_of_not_lt h450, h460⟩⟩
+        by_cases h470: n < 470; exact fixed_func_col_14_460_to_469_input c ⟨n, Finset.mem_Ico.mpr ⟨Nat.le_of_not_lt h460, h470⟩⟩
+        by_cases h480: n < 480; exact fixed_func_col_14_470_to_479_input c ⟨n, Finset.mem_Ico.mpr ⟨Nat.le_of_not_lt h470, h480⟩⟩
+        by_cases h490: n < 490; exact fixed_func_col_14_480_to_489_input c ⟨n, Finset.mem_Ico.mpr ⟨Nat.le_of_not_lt h480, h490⟩⟩
+        exact fixed_func_col_14_490_to_499_input c ⟨n, Finset.mem_Ico.mpr ⟨Nat.le_of_not_lt h490, h500⟩⟩
+      by_cases h600: n < 600
+      . by_cases h510: n < 510; exact fixed_func_col_14_500_to_509_input c ⟨n, Finset.mem_Ico.mpr ⟨Nat.le_of_not_lt h500, h510⟩⟩
+        by_cases h520: n < 520; exact fixed_func_col_14_510_to_519_input c ⟨n, Finset.mem_Ico.mpr ⟨Nat.le_of_not_lt h510, h520⟩⟩
+        by_cases h530: n < 530; exact fixed_func_col_14_520_to_529_input c ⟨n, Finset.mem_Ico.mpr ⟨Nat.le_of_not_lt h520, h530⟩⟩
+        by_cases h540: n < 540; exact fixed_func_col_14_530_to_539_input c ⟨n, Finset.mem_Ico.mpr ⟨Nat.le_of_not_lt h530, h540⟩⟩
+        by_cases h550: n < 550; exact fixed_func_col_14_540_to_549_input c ⟨n, Finset.mem_Ico.mpr ⟨Nat.le_of_not_lt h540, h550⟩⟩
+        by_cases h560: n < 560; exact fixed_func_col_14_550_to_559_input c ⟨n, Finset.mem_Ico.mpr ⟨Nat.le_of_not_lt h550, h560⟩⟩
+        by_cases h570: n < 570; exact fixed_func_col_14_560_to_569_input c ⟨n, Finset.mem_Ico.mpr ⟨Nat.le_of_not_lt h560, h570⟩⟩
+        by_cases h580: n < 580; exact fixed_func_col_14_570_to_579_input c ⟨n, Finset.mem_Ico.mpr ⟨Nat.le_of_not_lt h570, h580⟩⟩
+        by_cases h590: n < 590; exact fixed_func_col_14_580_to_589_input c ⟨n, Finset.mem_Ico.mpr ⟨Nat.le_of_not_lt h580, h590⟩⟩
+        exact fixed_func_col_14_590_to_599_input c ⟨n, Finset.mem_Ico.mpr ⟨Nat.le_of_not_lt h590, h600⟩⟩
+      by_cases h610: n < 610; exact fixed_func_col_14_600_to_609_input c ⟨n, Finset.mem_Ico.mpr ⟨Nat.le_of_not_lt h600, h610⟩⟩
+      by_cases h620: n < 620; exact fixed_func_col_14_610_to_619_input c ⟨n, Finset.mem_Ico.mpr ⟨Nat.le_of_not_lt h610, h620⟩⟩
+      exact fixed_func_col_14_620_to_624_input c ⟨n, Finset.mem_Ico.mpr ⟨Nat.le_of_not_lt h620, hn⟩⟩
+
+  lemma fixed_func_col_14_eq_input_of_lt_usable_rows (c: ValidCircuit P P_Prime) (n: ℕ) (hn: n < c.usable_rows):
+    fixed_func_col_14 c n = input_by_row P (if n < 625 then n else 0) := by
+      split
+      case isTrue h => exact fixed_func_col_14_0_to_624_input c ⟨n, h⟩
+      case isFalse h =>
+        unfold fixed_func_col_14
+        rewrite [
+          if_neg (by omega),
+          if_neg (by omega),
+          if_neg (by omega),
+          if_neg (by omega),
+          if_pos (by omega)
+        ]
+        simp [input_by_row, input]
+
+end Keccak.Lookups.ChiBase
