Examples/Scroll/Keccak/Lookups/PackTable/Lookups.lean
@@ -1,0 +1,39 @@
+import Examples.Scroll.Keccak.Lookups.PackTable.Packed
+import Examples.Scroll.Keccak.Lookups.PackTable.Unpacked
+
+namespace Keccak.Lookups.PackTable
+
+  lemma lookup_pack_table (col1 col2: ℕ)
+    (c: ValidCircuit P P_Prime) (hlookup: ∀ row < c.usable_rows,
+      ∃ lookup_row < c.usable_rows,
+      (c.get_advice col1 row, c.get_advice col2 row) =
+      (c.get_fixed 17 lookup_row, c.get_fixed 16 lookup_row)
+    ) (h_fixed: c.1.Fixed = fixed_func c):
+    ∀ row < c.usable_rows, ∃ x: ℕ,
+      x < 256 ∧
+      c.get_advice col1 row = pack P (into_bits [x]) ∧
+      c.get_advice col2 row = x
+    := by
+      intro row hrow
+      obtain ⟨lookup_row, ⟨hlookup_row, hlookup⟩⟩ := hlookup row hrow
+      by_cases hlookup_row_range: lookup_row < 256
+      all_goals simp_all [ValidCircuit.get_fixed, fixed_func, fixed_func_col_16_eq_unpacked_of_lt_usable_rows, fixed_func_col_17_eq_packed_of_lt_usable_rows, pack, pack_with_base, keccak_constants, into_bits, loop_8]
+      . use lookup_row
+      . use 0
+        norm_num
+
+  lemma lookup_1_pack_table (c: ValidCircuit P P_Prime) (hlookup: lookup_1 c) (h_fixed: c.1.Fixed = fixed_func c):
+    ∀ row < c.usable_rows, ∃ x: ℕ,
+      x < 256 ∧
+      c.get_advice 12 row = pack P (into_bits [x]) ∧
+      c.get_advice 13 row = x
+    := lookup_pack_table 12 13 c hlookup h_fixed
+
+  lemma lookup_86_pack_table (c: ValidCircuit P P_Prime) (hlookup: lookup_86 c) (h_fixed: c.1.Fixed = fixed_func c):
+    ∀ row < c.usable_rows, ∃ x: ℕ,
+      x < 256 ∧
+      c.get_advice 146 row = pack P (into_bits [x]) ∧
+      c.get_advice 147 row = x
+    := lookup_pack_table 146 147 c hlookup h_fixed
+
+end Keccak.Lookups.PackTable
