Examples/Scroll/Keccak/Lookups/PackTable/Unpacked.lean
@@ -1,0 +1,106 @@
+import Examples.Scroll.Keccak.Constants
+
+namespace Keccak.Lookups.PackTable
+  -- columns 16 and 17
+
+  lemma fixed_func_col_16_0_to_9_unpacked (c: ValidCircuit P P_Prime) (n: Finset.Ico 0 10): fixed_func_col_16 c n = n := by
+    fin_cases n <;> simp [fixed_func_col_16, fixed_func_col_16_0_to_99, fixed_func_col_16_0_to_9]
+  lemma fixed_func_col_16_10_to_19_unpacked (c: ValidCircuit P P_Prime) (n: Finset.Ico 10 20): fixed_func_col_16 c n = n := by
+    fin_cases n <;> simp [fixed_func_col_16, fixed_func_col_16_0_to_99, fixed_func_col_16_10_to_19]
+  lemma fixed_func_col_16_20_to_29_unpacked (c: ValidCircuit P P_Prime) (n: Finset.Ico 20 30): fixed_func_col_16 c n = n := by
+    fin_cases n <;> simp [fixed_func_col_16, fixed_func_col_16_0_to_99, fixed_func_col_16_20_to_29]
+  lemma fixed_func_col_16_30_to_39_unpacked (c: ValidCircuit P P_Prime) (n: Finset.Ico 30 40): fixed_func_col_16 c n = n := by
+    fin_cases n <;> simp [fixed_func_col_16, fixed_func_col_16_0_to_99, fixed_func_col_16_30_to_39]
+  lemma fixed_func_col_16_40_to_49_unpacked (c: ValidCircuit P P_Prime) (n: Finset.Ico 40 50): fixed_func_col_16 c n = n := by
+    fin_cases n <;> simp [fixed_func_col_16, fixed_func_col_16_0_to_99, fixed_func_col_16_40_to_49]
+  lemma fixed_func_col_16_50_to_59_unpacked (c: ValidCircuit P P_Prime) (n: Finset.Ico 50 60): fixed_func_col_16 c n = n := by
+    fin_cases n <;> simp [fixed_func_col_16, fixed_func_col_16_0_to_99, fixed_func_col_16_50_to_59]
+  lemma fixed_func_col_16_60_to_69_unpacked (c: ValidCircuit P P_Prime) (n: Finset.Ico 60 70): fixed_func_col_16 c n = n := by
+    fin_cases n <;> simp [fixed_func_col_16, fixed_func_col_16_0_to_99, fixed_func_col_16_60_to_69]
+  lemma fixed_func_col_16_70_to_79_unpacked (c: ValidCircuit P P_Prime) (n: Finset.Ico 70 80): fixed_func_col_16 c n = n := by
+    fin_cases n <;> simp [fixed_func_col_16, fixed_func_col_16_0_to_99, fixed_func_col_16_70_to_79]
+  lemma fixed_func_col_16_80_to_89_unpacked (c: ValidCircuit P P_Prime) (n: Finset.Ico 80 90): fixed_func_col_16 c n = n := by
+    fin_cases n <;> simp [fixed_func_col_16, fixed_func_col_16_0_to_99, fixed_func_col_16_80_to_89]
+  lemma fixed_func_col_16_90_to_99_unpacked (c: ValidCircuit P P_Prime) (n: Finset.Ico 90 100): fixed_func_col_16 c n = n := by
+    fin_cases n <;> simp [fixed_func_col_16, fixed_func_col_16_0_to_99, fixed_func_col_16_90_to_99]
+  lemma fixed_func_col_16_100_to_109_unpacked (c: ValidCircuit P P_Prime) (n: Finset.Ico 100 110): fixed_func_col_16 c n = n := by
+    fin_cases n <;> simp [fixed_func_col_16, fixed_func_col_16_100_to_199, fixed_func_col_16_100_to_109]
+  lemma fixed_func_col_16_110_to_119_unpacked (c: ValidCircuit P P_Prime) (n: Finset.Ico 110 120): fixed_func_col_16 c n = n := by
+    fin_cases n <;> simp [fixed_func_col_16, fixed_func_col_16_100_to_199, fixed_func_col_16_110_to_119]
+  lemma fixed_func_col_16_120_to_129_unpacked (c: ValidCircuit P P_Prime) (n: Finset.Ico 120 130): fixed_func_col_16 c n = n := by
+    fin_cases n <;> simp [fixed_func_col_16, fixed_func_col_16_100_to_199, fixed_func_col_16_120_to_129]
+  lemma fixed_func_col_16_130_to_139_unpacked (c: ValidCircuit P P_Prime) (n: Finset.Ico 130 140): fixed_func_col_16 c n = n := by
+    fin_cases n <;> simp [fixed_func_col_16, fixed_func_col_16_100_to_199, fixed_func_col_16_130_to_139]
+  lemma fixed_func_col_16_140_to_149_unpacked (c: ValidCircuit P P_Prime) (n: Finset.Ico 140 150): fixed_func_col_16 c n = n := by
+    fin_cases n <;> simp [fixed_func_col_16, fixed_func_col_16_100_to_199, fixed_func_col_16_140_to_149]
+  lemma fixed_func_col_16_150_to_159_unpacked (c: ValidCircuit P P_Prime) (n: Finset.Ico 150 160): fixed_func_col_16 c n = n := by
+    fin_cases n <;> simp [fixed_func_col_16, fixed_func_col_16_100_to_199, fixed_func_col_16_150_to_159]
+  lemma fixed_func_col_16_160_to_169_unpacked (c: ValidCircuit P P_Prime) (n: Finset.Ico 160 170): fixed_func_col_16 c n = n := by
+    fin_cases n <;> simp [fixed_func_col_16, fixed_func_col_16_100_to_199, fixed_func_col_16_160_to_169]
+  lemma fixed_func_col_16_170_to_179_unpacked (c: ValidCircuit P P_Prime) (n: Finset.Ico 170 180): fixed_func_col_16 c n = n := by
+    fin_cases n <;> simp [fixed_func_col_16, fixed_func_col_16_100_to_199, fixed_func_col_16_170_to_179]
+  lemma fixed_func_col_16_180_to_189_unpacked (c: ValidCircuit P P_Prime) (n: Finset.Ico 180 190): fixed_func_col_16 c n = n := by
+    fin_cases n <;> simp [fixed_func_col_16, fixed_func_col_16_100_to_199, fixed_func_col_16_180_to_189]
+  lemma fixed_func_col_16_190_to_199_unpacked (c: ValidCircuit P P_Prime) (n: Finset.Ico 190 200): fixed_func_col_16 c n = n := by
+    fin_cases n <;> simp [fixed_func_col_16, fixed_func_col_16_100_to_199, fixed_func_col_16_190_to_199]
+  lemma fixed_func_col_16_200_to_209_unpacked (c: ValidCircuit P P_Prime) (n: Finset.Ico 200 210): fixed_func_col_16 c n = n := by
+    fin_cases n <;> simp [fixed_func_col_16, fixed_func_col_16_200_to_254, fixed_func_col_16_200_to_209]
+  lemma fixed_func_col_16_210_to_219_unpacked (c: ValidCircuit P P_Prime) (n: Finset.Ico 210 220): fixed_func_col_16 c n = n := by
+    fin_cases n <;> simp [fixed_func_col_16, fixed_func_col_16_200_to_254, fixed_func_col_16_210_to_219]
+  lemma fixed_func_col_16_220_to_229_unpacked (c: ValidCircuit P P_Prime) (n: Finset.Ico 220 230): fixed_func_col_16 c n = n := by
+    fin_cases n <;> simp [fixed_func_col_16, fixed_func_col_16_200_to_254, fixed_func_col_16_220_to_229]
+  lemma fixed_func_col_16_230_to_239_unpacked (c: ValidCircuit P P_Prime) (n: Finset.Ico 230 240): fixed_func_col_16 c n = n := by
+    fin_cases n <;> simp [fixed_func_col_16, fixed_func_col_16_200_to_254, fixed_func_col_16_230_to_239]
+  lemma fixed_func_col_16_240_to_249_unpacked (c: ValidCircuit P P_Prime) (n: Finset.Ico 240 250): fixed_func_col_16 c n = n := by
+    fin_cases n <;> simp [fixed_func_col_16, fixed_func_col_16_200_to_254, fixed_func_col_16_240_to_249]
+  lemma fixed_func_col_16_250_to_255_unpacked (c: ValidCircuit P P_Prime) (n: Finset.Ico 250 256): fixed_func_col_16 c n = n := by
+    fin_cases n <;> simp [fixed_func_col_16, fixed_func_col_16_200_to_254]
+
+  lemma fixed_func_col_16_0_to_255_unpacked (c : ValidCircuit P P_Prime) (n : Fin 256) :
+    fixed_func_col_16 c n = n := by
+      rcases n with ⟨n, hn⟩
+      by_cases h100: n < 100
+      . by_cases h10: n < 10; exact fixed_func_col_16_0_to_9_unpacked c ⟨n, Finset.mem_Ico.mpr ⟨(Nat.zero_le n), h10⟩⟩
+        by_cases h20: n < 20; exact fixed_func_col_16_10_to_19_unpacked c ⟨n, Finset.mem_Ico.mpr ⟨Nat.le_of_not_lt h10, h20⟩⟩
+        by_cases h30: n < 30; exact fixed_func_col_16_20_to_29_unpacked c ⟨n, Finset.mem_Ico.mpr ⟨Nat.le_of_not_lt h20, h30⟩⟩
+        by_cases h40: n < 40; exact fixed_func_col_16_30_to_39_unpacked c ⟨n, Finset.mem_Ico.mpr ⟨Nat.le_of_not_lt h30, h40⟩⟩
+        by_cases h50: n < 50; exact fixed_func_col_16_40_to_49_unpacked c ⟨n, Finset.mem_Ico.mpr ⟨Nat.le_of_not_lt h40, h50⟩⟩
+        by_cases h60: n < 60; exact fixed_func_col_16_50_to_59_unpacked c ⟨n, Finset.mem_Ico.mpr ⟨Nat.le_of_not_lt h50, h60⟩⟩
+        by_cases h70: n < 70; exact fixed_func_col_16_60_to_69_unpacked c ⟨n, Finset.mem_Ico.mpr ⟨Nat.le_of_not_lt h60, h70⟩⟩
+        by_cases h80: n < 80; exact fixed_func_col_16_70_to_79_unpacked c ⟨n, Finset.mem_Ico.mpr ⟨Nat.le_of_not_lt h70, h80⟩⟩
+        by_cases h90: n < 90; exact fixed_func_col_16_80_to_89_unpacked c ⟨n, Finset.mem_Ico.mpr ⟨Nat.le_of_not_lt h80, h90⟩⟩
+        exact fixed_func_col_16_90_to_99_unpacked c ⟨n, Finset.mem_Ico.mpr ⟨Nat.le_of_not_lt h90, h100⟩⟩
+      by_cases h200: n < 200
+      . by_cases h110: n < 110; exact fixed_func_col_16_100_to_109_unpacked c ⟨n, Finset.mem_Ico.mpr ⟨Nat.le_of_not_lt h100, h110⟩⟩
+        by_cases h120: n < 120; exact fixed_func_col_16_110_to_119_unpacked c ⟨n, Finset.mem_Ico.mpr ⟨Nat.le_of_not_lt h110, h120⟩⟩
+        by_cases h130: n < 130; exact fixed_func_col_16_120_to_129_unpacked c ⟨n, Finset.mem_Ico.mpr ⟨Nat.le_of_not_lt h120, h130⟩⟩
+        by_cases h140: n < 140; exact fixed_func_col_16_130_to_139_unpacked c ⟨n, Finset.mem_Ico.mpr ⟨Nat.le_of_not_lt h130, h140⟩⟩
+        by_cases h150: n < 150; exact fixed_func_col_16_140_to_149_unpacked c ⟨n, Finset.mem_Ico.mpr ⟨Nat.le_of_not_lt h140, h150⟩⟩
+        by_cases h160: n < 160; exact fixed_func_col_16_150_to_159_unpacked c ⟨n, Finset.mem_Ico.mpr ⟨Nat.le_of_not_lt h150, h160⟩⟩
+        by_cases h170: n < 170; exact fixed_func_col_16_160_to_169_unpacked c ⟨n, Finset.mem_Ico.mpr ⟨Nat.le_of_not_lt h160, h170⟩⟩
+        by_cases h180: n < 180; exact fixed_func_col_16_170_to_179_unpacked c ⟨n, Finset.mem_Ico.mpr ⟨Nat.le_of_not_lt h170, h180⟩⟩
+        by_cases h190: n < 190; exact fixed_func_col_16_180_to_189_unpacked c ⟨n, Finset.mem_Ico.mpr ⟨Nat.le_of_not_lt h180, h190⟩⟩
+        exact fixed_func_col_16_190_to_199_unpacked c ⟨n, Finset.mem_Ico.mpr ⟨Nat.le_of_not_lt h190, h200⟩⟩
+      by_cases h210: n < 210; exact fixed_func_col_16_200_to_209_unpacked c ⟨n, Finset.mem_Ico.mpr ⟨Nat.le_of_not_lt h200, h210⟩⟩
+      by_cases h220: n < 220; exact fixed_func_col_16_210_to_219_unpacked c ⟨n, Finset.mem_Ico.mpr ⟨Nat.le_of_not_lt h210, h220⟩⟩
+      by_cases h230: n < 230; exact fixed_func_col_16_220_to_229_unpacked c ⟨n, Finset.mem_Ico.mpr ⟨Nat.le_of_not_lt h220, h230⟩⟩
+      by_cases h240: n < 240; exact fixed_func_col_16_230_to_239_unpacked c ⟨n, Finset.mem_Ico.mpr ⟨Nat.le_of_not_lt h230, h240⟩⟩
+      by_cases h250: n < 250; exact fixed_func_col_16_240_to_249_unpacked c ⟨n, Finset.mem_Ico.mpr ⟨Nat.le_of_not_lt h240, h250⟩⟩
+      exact fixed_func_col_16_250_to_255_unpacked c ⟨n, Finset.mem_Ico.mpr ⟨Nat.le_of_not_lt h250, hn⟩⟩
+
+  lemma fixed_func_col_16_eq_unpacked_of_lt_usable_rows (c: ValidCircuit P P_Prime) (n: ℕ) (hn: n < c.usable_rows):
+    fixed_func_col_16 c n = if n < 256 then n else 0 := by
+      split
+      case isTrue h => exact fixed_func_col_16_0_to_255_unpacked c ⟨n, h⟩
+      case isFalse h =>
+        unfold fixed_func_col_16
+        rewrite [
+          if_neg (by omega),
+          if_neg (by omega),
+          if_neg (by omega),
+          if_neg (by omega),
+          if_pos (by omega)
+        ]
+        simp
+
+end Keccak.Lookups.PackTable
